Moved hoising to different file and proved that it's in the reflexive transitive closure of a rewrite relation. Also, bit of indentation at cps_util

theories/L6_PCPS/cps_util.v
@@ -18,12 +18,12 @@ Require Import cps.
 
  *)
 
- Ltac destructAll :=
-   match goal with
-     | [ H : _ /\ _ |- _] => destruct H; destructAll
-     | [ H : exists E, _ |- _ ] => destruct H; destructAll
-     | _ => subst
-   end.
+Ltac destructAll :=
+  match goal with
+    | [ H : _ /\ _ |- _] => destruct H; destructAll
+    | [ H : exists E, _ |- _ ] => destruct H; destructAll
+    | _ => subst
+  end.
 
 
 Definition var_dec := M.elt_eq.
@@ -33,18 +33,18 @@ Section SUBTERM.
 
 
   Inductive subterm_e: exp -> exp -> Prop :=
-    (* immediate *)
-    | subterm_constr: forall x t c ys e,  subterm_e e (Econstr x t c ys e)
-    | subterm_proj: forall v t n y e, subterm_e e (Eproj v t n y e)
-    | subterm_prim: forall x t f ys e, subterm_e e (Eprim x t f ys e)
-    (* remote *)
-    | subterm_constr': forall x t c ys e e', subterm_e e' e -> subterm_e e' (Econstr x t c ys e)
-    | subterm_proj': forall v t n y e e', subterm_e e' e -> subterm_e e' (Eproj v t n y e)
-    | subterm_prim': forall x t f ys e e', subterm_e e' e -> subterm_e e' (Eprim x t f ys e)
+  (* immediate *)
+  | subterm_constr: forall x t c ys e,  subterm_e e (Econstr x t c ys e)
+  | subterm_proj: forall v t n y e, subterm_e e (Eproj v t n y e)
+  | subterm_prim: forall x t f ys e, subterm_e e (Eprim x t f ys e)
+  (* remote *)
+  | subterm_constr': forall x t c ys e e', subterm_e e' e -> subterm_e e' (Econstr x t c ys e)
+  | subterm_proj': forall v t n y e e', subterm_e e' e -> subterm_e e' (Eproj v t n y e)
+  | subterm_prim': forall x t f ys e e', subterm_e e' e -> subterm_e e' (Eprim x t f ys e)
   (* in fdefs *)
-    | subterm_fds: forall e' fds e,
-        subterm_fds_e e' fds ->
-        subterm_e e' (Efun fds e)
+  | subterm_fds: forall e' fds e,
+                   subterm_fds_e e' fds ->
+                   subterm_e e' (Efun fds e)
   with subterm_fds_e: exp -> fundefs -> Prop :=
        | subterm_cons: forall e f t ys fds', subterm_fds_e e (Fcons f t ys e fds')
        | subterm_cons': forall e' e f t ys fds', subterm_e e' e -> subterm_fds_e e' (Fcons f t ys e fds')
@@ -56,27 +56,27 @@ Section SUBTERM.
   | subfds_cons: forall fds f t ys e, subfds_fds fds (Fcons f t ys e fds).
 
 
-Definition subterm_or_eq: exp -> exp -> Prop :=
-   fun e' e => subterm_e e' e \/ e' = e.
+  Definition subterm_or_eq: exp -> exp -> Prop :=
+    fun e' e => subterm_e e' e \/ e' = e.
 
-Definition subfds_or_eq: fundefs -> fundefs -> Prop :=
-  fun fds' fds => subfds_fds fds' fds \/ fds' = fds.
+  Definition subfds_or_eq: fundefs -> fundefs -> Prop :=
+    fun fds' fds => subfds_fds fds' fds \/ fds' = fds.
 
-Definition subfds_e: fundefs -> exp -> Prop := 
+  Definition subfds_e: fundefs -> exp -> Prop := 
     fun fds  e => exists fds' e', subterm_or_eq (Efun fds' e') e /\  subfds_or_eq fds fds'.
 
-Definition subfds_or_eq_left: forall fds' fds fds'', subfds_fds fds fds' -> subfds_or_eq fds' fds'' -> subfds_or_eq fds fds''.
-Proof.
-  induction fds'; intros.
-  - inversion H; subst. eapply IHfds'. apply H3. admit. admit.
-Admitted.  
+  Definition subfds_or_eq_left: forall fds' fds fds'', subfds_fds fds fds' -> subfds_or_eq fds' fds'' -> subfds_or_eq fds fds''.
+  Proof.
+    induction fds'; intros.
+    - inversion H; subst. eapply IHfds'. apply H3. admit. admit.
+  Admitted.  
 
-Theorem subfds_e_subfds: forall fds e fds', subfds_fds fds' fds -> subfds_e fds e -> subfds_e fds' e.
-Proof.
-  destruct fds; intros.
-  - destruct H0; destructAll. exists x. exists x0. split. assumption.  eapply subfds_or_eq_left. apply H. assumption.
-  - inversion H. 
-Qed.
+  Theorem subfds_e_subfds: forall fds e fds', subfds_fds fds' fds -> subfds_e fds e -> subfds_e fds' e.
+  Proof.
+    destruct fds; intros.
+    - destruct H0; destructAll. exists x. exists x0. split. assumption.  eapply subfds_or_eq_left. apply H. assumption.
+    - inversion H. 
+  Qed.
 
 End SUBTERM.
 
@@ -92,34 +92,34 @@ Section CTX.
   with fundefs_ctx :=
        | Fcons1_c:  var -> type -> list var -> exp_ctx -> fundefs -> fundefs_ctx
        | Fcons2_c:  var -> type -> list var -> exp -> fundefs_ctx -> fundefs_ctx.
- 
+  
 
 
 
   Inductive app_ctx: exp_ctx -> exp -> exp -> Prop :=
   | Hole_ac: forall e, app_ctx Hole_c e e
   | Constr_ac : forall x t k c ys e ce,
-           app_ctx c e ce ->        
-           app_ctx (Econstr_c x t k ys c) e (Econstr x t k ys ce)
+                  app_ctx c e ce ->        
+                  app_ctx (Econstr_c x t k ys c) e (Econstr x t k ys ce)
   | Proj_ac : forall x t n y e c ce, 
-           app_ctx c e ce ->        
-           app_ctx (Eproj_c x t n y c) e (Eproj x t n y ce)
+                app_ctx c e ce ->        
+                app_ctx (Eproj_c x t n y c) e (Eproj x t n y ce)
   | Prim_ac : forall x t f ys e c ce, 
                 app_ctx c e ce ->        
                 app_ctx (Eprim_c x t f ys c) e (Eprim x t f ys ce)
   | Fun1_ac : forall c e ce fds,
-      app_ctx c e ce ->
-      app_ctx (Efun1_c fds c) e (Efun fds ce)
+                app_ctx c e ce ->
+                app_ctx (Efun1_c fds c) e (Efun fds ce)
   | Fun2_ac : forall e cfds cfdse e',
-       app_f_ctx cfds e cfdse ->          
-       app_ctx (Efun2_c cfds e') e (Efun cfdse e')
+                app_f_ctx cfds e cfdse ->          
+                app_ctx (Efun2_c cfds e') e (Efun cfdse e')
   with app_f_ctx : fundefs_ctx -> exp -> fundefs -> Prop :=
        | Fcons1_ac : forall c e ce f t ys fds,
-           app_ctx c e ce -> 
-           app_f_ctx (Fcons1_c f t ys c fds) e (Fcons f t ys ce fds)
+                       app_ctx c e ce -> 
+                       app_f_ctx (Fcons1_c f t ys c fds) e (Fcons f t ys ce fds)
        | Fcons2_ac: forall e cfdse f cfds ys e' t, 
-           app_f_ctx cfds e cfdse -> 
-           app_f_ctx (Fcons2_c f t ys e' cfds) e (Fcons f t ys e' cfdse)
+                      app_f_ctx cfds e cfdse -> 
+                      app_f_ctx (Fcons2_c f t ys e' cfds) e (Fcons f t ys e' cfdse)
   .
   
   Hint Constructors app_ctx app_f_ctx.
@@ -137,39 +137,37 @@ Section CTX.
          match c with
            | Fcons1_c f t ys c fds => Fcons f t ys (app_ctx_f c e) fds
            | Fcons2_c f t ys e' cfds => Fcons f t ys e' (app_f_ctx_f cfds e)
-         end
-  .
+         end.
   
-Inductive  comp_ctx: exp_ctx -> exp_ctx -> exp_ctx -> Prop :=
+  Inductive  comp_ctx: exp_ctx -> exp_ctx -> exp_ctx -> Prop :=
   | Hole_cc: forall e, comp_ctx Hole_c e e
   | Constr_cc : forall x t k c ys e ce,
-           comp_ctx c e ce ->        
-           comp_ctx (Econstr_c x t k ys c) e (Econstr_c x t k ys ce)
+                  comp_ctx c e ce ->        
+                  comp_ctx (Econstr_c x t k ys c) e (Econstr_c x t k ys ce)
   | Proj_cc : forall x t n y e c ce, 
-           comp_ctx c e ce ->        
-           comp_ctx (Eproj_c x t n y c) e (Eproj_c x t n y ce)
+                comp_ctx c e ce ->        
+                comp_ctx (Eproj_c x t n y c) e (Eproj_c x t n y ce)
   | Prim_cc : forall x t f ys e c ce, 
                 comp_ctx c e ce ->        
                 comp_ctx (Eprim_c x t f ys c) e (Eprim_c x t f ys ce)
   | Fun1_cc : forall c e ce fds,
-      comp_ctx c e ce ->
-      comp_ctx (Efun1_c fds c) e (Efun1_c fds ce)
+                comp_ctx c e ce ->
+                comp_ctx (Efun1_c fds c) e (Efun1_c fds ce)
   | Fun2_cc : forall e cfds cfdse e',
-       comp_f_ctx cfds e cfdse ->          
-       comp_ctx (Efun2_c cfds e') e (Efun2_c cfdse e')
+                comp_f_ctx cfds e cfdse ->          
+                comp_ctx (Efun2_c cfds e') e (Efun2_c cfdse e')
   with comp_f_ctx : fundefs_ctx -> exp_ctx -> fundefs_ctx -> Prop :=
        | Fcons1_cc : forall c e ce f t ys fds,
-           comp_ctx c e ce -> 
-           comp_f_ctx (Fcons1_c f t ys c fds) e (Fcons1_c f t ys ce fds)
+                       comp_ctx c e ce -> 
+                       comp_f_ctx (Fcons1_c f t ys c fds) e (Fcons1_c f t ys ce fds)
        | Fcons2_cc: forall e cfdse f cfds ys e' t, 
-           comp_f_ctx cfds e cfdse -> 
-           comp_f_ctx (Fcons2_c f t ys e' cfds) e (Fcons2_c f t ys e' cfdse)
-  .
+                      comp_f_ctx cfds e cfdse -> 
+                      comp_f_ctx (Fcons2_c f t ys e' cfds) e (Fcons2_c f t ys e' cfdse).
 
-    
   
-    Fixpoint comp_ctx_f (c1:exp_ctx) (c2:exp_ctx): exp_ctx :=
-        match c1 with
+  
+  Fixpoint comp_ctx_f (c1:exp_ctx) (c2:exp_ctx): exp_ctx :=
+    match c1 with
       | Hole_c => c2
       | Econstr_c x t k ys c => Econstr_c x t k ys (comp_ctx_f c c2)
       | Eproj_c x t n y c => Eproj_c x t n y (comp_ctx_f c c2)
@@ -192,25 +190,25 @@ Inductive  comp_ctx: exp_ctx -> exp_ctx -> exp_ctx -> Prop :=
     exists c, app_ctx c e' e.
 
 
-(* theorems about app and comp *)
-    Theorem app_ctx_f_correct: forall c e e',
+  (* theorems about app and comp *)
+  Theorem app_ctx_f_correct: forall c e e',
                                app_ctx_f c e  = e' <-> app_ctx c e e'
                                with app_f_ctx_f_correct: forall cf e e',
                                                            app_f_ctx_f cf e = e' <-> app_f_ctx cf e e'.
-      Admitted.
+  Admitted.
 
-    Theorem comp_ctx_f_correct: forall c c' cc',
-                                 comp_ctx_f c c'  = cc' <-> comp_ctx c c' cc'
-                                 with comp_f_ctx_f_correct: forall cf cf' ccf',
+  Theorem comp_ctx_f_correct: forall c c' cc',
+                                comp_ctx_f c c'  = cc' <-> comp_ctx c c' cc'
+                                with comp_f_ctx_f_correct: forall cf cf' ccf',
                                                              comp_f_ctx_f cf cf' = ccf' <-> comp_f_ctx cf cf' ccf'.
-    Admitted.
+  Admitted.
 
-    Theorem app_ctx_f_fuse : forall c c' e,
-                               app_ctx_f c (app_ctx_f c' e) = app_ctx_f (comp_ctx_f c c') e.
-      Admitted.
+  Theorem app_ctx_f_fuse : forall c c' e,
+                             app_ctx_f c (app_ctx_f c' e) = app_ctx_f (comp_ctx_f c c') e.
+  Admitted.
 
-    
-    
+  
+  
 
 
 End CTX.  
@@ -220,42 +218,42 @@ Section OCCUR.
   Definition num_occur_list (lv:list var) (v:var) : nat :=
     fold_right (fun v' n => if (var_dec v v') then 1 + n
                             else n) 0 lv.
-                                                       
-    
+  
+  
   
   (* number of time var occurs in exp (free or not) *)
   Inductive num_occur: exp -> var -> nat -> Prop :=
   | Num_occ_constr: forall x t c ys e v n, num_occur e v n -> num_occur (Econstr x t c ys e) v (n + (num_occur_list ys v))
   | Num_occ_prim: forall x t f ys e v n, num_occur e v n -> num_occur (Eprim x t f ys e) v (n + (num_occur_list ys v))
   | Num_occ_case: forall v' cl v,
-      num_occur (Ecase v' cl) v (num_occur_list (v'::(snd (split cl))) v)
+                    num_occur (Ecase v' cl) v (num_occur_list (v'::(snd (split cl))) v)
   | Num_occ_proj: forall e v n  y v' t n',
-      num_occur  e v n -> 
-      num_occur (Eproj v' t n' y e) v (num_occur_list [y] v + n)
+                    num_occur  e v n -> 
+                    num_occur (Eproj v' t n' y e) v (num_occur_list [y] v + n)
   | Num_occ_app: forall f ys v,
-      num_occur (Eapp f ys) v (num_occur_list (f::ys) v)
+                   num_occur (Eapp f ys) v (num_occur_list (f::ys) v)
   | Num_occ_fun: forall e v n m fl,
-      num_occur e v n ->
-      num_occur_fds fl v m ->
-      num_occur (Efun fl e) v (n + m )
+                   num_occur e v n ->
+                   num_occur_fds fl v m ->
+                   num_occur (Efun fl e) v (n + m )
   with num_occur_fds: fundefs -> var -> nat -> Prop :=
        | Num_occ_nil : forall v,
-           num_occur_fds Fnil v 0
+                         num_occur_fds Fnil v 0
        | Num_occ_cons : forall v t n v' ys e fds' m,
-                               num_occur e v n ->
-                               num_occur_fds fds' v m ->
-           num_occur_fds (Fcons v' t ys e fds') v (n + m).
+                          num_occur e v n ->
+                          num_occur_fds fds' v m ->
+                          num_occur_fds (Fcons v' t ys e fds') v (n + m).
 
 
-  (* number of time var occurs in a context *)
+  (* number of times var occurs in a context *)
   Inductive num_occur_ec: exp_ctx -> var -> nat -> Prop :=
   | Noec_hole: forall v, num_occur_ec Hole_c v 0
   | Noec_constr: forall c v n x t ys g,
-    num_occur_ec c v n -> 
-    num_occur_ec (Econstr_c x t g ys c) v (num_occur_list ys v + n)
+                   num_occur_ec c v n -> 
+                   num_occur_ec (Econstr_c x t g ys c) v (num_occur_list ys v + n)
   | Noec_prim: forall c v n x t f ys, 
-    num_occur_ec c v n -> 
-    num_occur_ec (Eprim_c x t f ys c) v (num_occur_list ys v + n )
+                 num_occur_ec c v n -> 
+                 num_occur_ec (Eprim_c x t f ys c) v (num_occur_list ys v + n )
   | Noec_proj: forall  v n y v' t n' c,
                  num_occur_ec c v n ->
                  num_occur_ec (Eproj_c v' t n' y c) v (num_occur_list [y] v + n)
@@ -269,61 +267,61 @@ Section OCCUR.
                  num_occur_ec (Efun2_c fdc e) v (n + m)
   with num_occur_fdc : fundefs_ctx -> var -> nat -> Prop :=
        | Nofc_fcons1 : forall v n m fds t ys c f,
-           num_occur_ec c v n ->
-           num_occur_fds fds v m -> 
-             num_occur_fdc (Fcons1_c f t ys c fds) v  (n + m)
+                         num_occur_ec c v n ->
+                         num_occur_fds fds v m -> 
+                         num_occur_fdc (Fcons1_c f t ys c fds) v  (n + m)
        | Nofc_fcons2 : forall e v n m fdc f t ys,
-           num_occur e v n ->
-           num_occur_fdc fdc v m ->
-           num_occur_fdc (Fcons2_c f t ys e fdc) v (n + m) 
+                         num_occur e v n ->
+                         num_occur_fdc fdc v m ->
+                         num_occur_fdc (Fcons2_c f t ys e fdc) v (n + m) 
   .
-                 
   
-    (* number of time var occurs in exp in an applied position *)
+  
+  (* number of times var occurs in exp in an applied position *)
   Inductive num_occur_app: exp -> var -> nat -> Prop :=
   | Num_oa_constr: forall x t c ys e v n, num_occur_app e v n -> num_occur_app (Econstr x t c ys e) v n
   | Num_oa_prim: forall x t f ys e v n, num_occur_app e v n -> num_occur_app (Eprim x t f ys e) v n
   | Num_oa_case: forall v' cl v,
-      num_occur_app (Ecase v' cl) v (num_occur_list [v'] v)
+                   num_occur_app (Ecase v' cl) v (num_occur_list [v'] v)
   | Num_oa_proj: forall e v n  y v' t n', (* TODO: A&J counts y here *)
-      num_occur_app  e v n -> 
-      num_occur_app (Eproj v' t n' y e) v (num_occur_list [y] v + n)
+                   num_occur_app  e v n -> 
+                   num_occur_app (Eproj v' t n' y e) v (num_occur_list [y] v + n)
   | Num_oa_app: forall f ys v,
-      num_occur_app (Eapp f ys) v (num_occur_list [f] v)
+                  num_occur_app (Eapp f ys) v (num_occur_list [f] v)
   | Num_oa_fun: forall e v n m fl,
-      num_occur_app e v n ->
-      num_occur_app_fds fl v m ->
-      num_occur_app (Efun fl e) v (n + m )
+                  num_occur_app e v n ->
+                  num_occur_app_fds fl v m ->
+                  num_occur_app (Efun fl e) v (n + m )
   with num_occur_app_fds: fundefs -> var -> nat -> Prop :=
        | Num_oa_nil : forall v,
-           num_occur_app_fds Fnil v 0
+                        num_occur_app_fds Fnil v 0
        | Num_oa_cons : forall v t n v' ys e fds' m,
-                               num_occur_app e v n ->
-                               num_occur_app_fds fds' v m ->
-           num_occur_app_fds (Fcons v' t ys e fds') v (n + m).
+                         num_occur_app e v n ->
+                         num_occur_app_fds fds' v m ->
+                         num_occur_app_fds (Fcons v' t ys e fds') v (n + m).
 
-    (* number of time var occurs in exp in an escaping position *)
+  (* number of times var occurs in exp in an escaping position *)
   Inductive num_occur_esc: exp -> var -> nat -> Prop :=
   | Num_oe_constr: forall x t c ys e v n, num_occur_esc e v n -> num_occur_esc (Econstr x t c ys e) v (n + (num_occur_list ys v))
   | Num_oe_prim: forall x t f ys e v n, num_occur_esc e v n -> num_occur_esc (Eprim x t f ys e) v (n + (num_occur_list ys v))
   | Num_oe_case: forall v' cl v,
-      num_occur_esc (Ecase v' cl) v (num_occur_list (snd (split cl)) v)
+                   num_occur_esc (Ecase v' cl) v (num_occur_list (snd (split cl)) v)
   | Num_oe_proj: forall e v n  y v' t n',
-      num_occur_esc  e v n -> 
-      num_occur_esc (Eproj v' t n' y e) v n
+                   num_occur_esc  e v n -> 
+                   num_occur_esc (Eproj v' t n' y e) v n
   | Num_oe_app: forall f ys v,
-      num_occur_esc (Eapp f ys) v (num_occur_list ys v)
+                  num_occur_esc (Eapp f ys) v (num_occur_list ys v)
   | Num_oe_fun: forall e v n m fl,
-      num_occur_esc e v n ->
-      num_occur_esc_fds fl v m ->
-      num_occur_esc (Efun fl e) v (n + m )
+                  num_occur_esc e v n ->
+                  num_occur_esc_fds fl v m ->
+                  num_occur_esc (Efun fl e) v (n + m )
   with num_occur_esc_fds: fundefs -> var -> nat -> Prop :=
        | Num_oe_nil : forall v,
-           num_occur_esc_fds Fnil v 0
+                        num_occur_esc_fds Fnil v 0
        | Num_oe_cons : forall v t n v' ys e fds' m,
-                               num_occur_esc e v n ->
-                               num_occur_esc_fds fds' v m ->
-           num_occur_esc_fds (Fcons v' t ys e fds') v (n + m).
+                         num_occur_esc e v n ->
+                         num_occur_esc_fds fds' v m ->
+                         num_occur_esc_fds (Fcons v' t ys e fds') v (n + m).
 
 
 
@@ -347,14 +345,14 @@ Section BINDING.
                                               bv_f (Fcons f t ys e fds) (f::(ys++(l1++l2)))
        | Nil_bv : bv_f Fnil [].
 
-Hint Constructors bv_e bv_f.
+  Hint Constructors bv_e bv_f.
   
-Theorem e_bv_e : forall e, exists l, bv_e e l
-with e_bv_f: forall f, exists l, bv_f f l.
+  Theorem e_bv_e : forall e, exists l, bv_e e l
+                                       with e_bv_f: forall f, exists l, bv_f f l.
   Proof.
     induction e; destructAll; clear e_bv_e; eauto. specialize (e_bv_f f). destruct e_bv_f. eauto. 
     induction f; destructAll; clear e_bv_f; eauto.  specialize (e_bv_e e); destruct e_bv_e. eauto.
-Qed.
+  Qed.
 
 
   
@@ -371,22 +369,22 @@ Qed.
       + specialize (bv_e_det e _ _ H7 H15); specialize (IHf _ _ H8 H16); subst; reflexivity.
       + reflexivity.
   Qed.
-*)
- 
+ *)
+  
 
   
 End BINDING.
 
 Section OTHER.
 
- Theorem findtag_not_empty: forall A cl (k:A) (v:tag), findtag cl v = Some k -> 0 < (length cl).
- Proof.
-   induction cl; intros.
-   - inversion H.
-   - simpl in H. destruct a. destruct (M.elt_eq t v).
-     + inversion H. simpl. omega.
-     + simpl. apply IHcl in H. omega.
- Qed.
+  Theorem findtag_not_empty: forall A cl (k:A) (v:tag), findtag cl v = Some k -> 0 < (length cl).
+  Proof.
+    induction cl; intros.
+    - inversion H.
+    - simpl in H. destruct a. destruct (M.elt_eq t v).
+      + inversion H. simpl. omega.
+      + simpl. apply IHcl in H. omega.
+  Qed.
 
- 
+  
 End OTHER.  
