theories/L6_PCPS/hoisting.v
@@ -1,0 +1,345 @@
+Require Import cps cps_util shrink_cps.
+Require Import BinNat Relations.
+
+(* TODO : move dependencies from shrink_cps to common file *)
+
+Fixpoint exp_hoist (e : exp) (defs : fundefs ) (f : exp -> exp) : exp :=
+  match e with
+    | Econstr x typ tag ys e' =>
+      exp_hoist e' defs (fun e => f (Econstr x typ tag ys e))
+    | Ecase x xs =>
+      Efun defs (f (Ecase x xs))
+    | Eproj x typ n y e' =>
+      exp_hoist e' defs (fun e => f (Eproj x typ n y e))
+    | Efun fdefs e =>
+      let defs' := fundefs_hoist fdefs defs id in
+      exp_hoist e defs' f 
+    | Eapp g xs =>
+      Efun defs (f (Eapp g xs))
+    | Eprim x typ prim ys e' =>
+      exp_hoist e' defs (fun e => f (Eprim x typ prim ys e))
+  end
+with fundefs_hoist (defs hdefs : fundefs) (f : fundefs -> fundefs) :
+       fundefs :=
+  match defs with 
+    | Fcons g t xs e defs =>
+      match exp_hoist e hdefs id with
+        | Efun hdefs' e' =>
+          fundefs_hoist defs hdefs' (fun d => f (Fcons g t xs e' d)) 
+        | _ => hdefs
+      end
+    | Fnil => f hdefs 
+  end.
+
+(** expressions without function definitions *)
+Inductive no_fun : exp -> Prop  :=
+| Econstr_no_fun :
+    forall x tau t xs e,
+      no_fun e ->
+      no_fun (Econstr x tau t xs e)
+| Ecase_no_fun :
+    forall x txs, no_fun (Ecase x txs)
+| Eproj_no_fun :
+    forall x tau n y e,
+      no_fun e ->
+      no_fun (Eproj x tau n y e)
+| Eapp_no_fun :
+    forall x ys, no_fun (Eapp x ys)
+| Eprim_no_fun :
+    forall x tau p xs e,
+      no_fun e ->
+      no_fun (Eprim x tau p xs e).
+
+(** function definitions without nested function definitions *)
+Inductive no_fun_defs : fundefs -> Prop  :=
+| Fcons_no_fun :
+    forall f tau xs e defs,
+      no_fun e ->
+      no_fun_defs defs ->
+      no_fun_defs (Fcons f tau xs e defs)
+| Fnil_no_fun :
+    no_fun_defs Fnil.
+
+Hint Constructors no_fun no_fun_defs.
+
+(** hoisting as a rewrite relation *)
+Inductive hoist_rw : relation exp :=
+| hoist1 :
+    forall e1 e2 defs defs' defs'' e c,
+      split_fds defs defs' defs'' ->
+      no_fun_defs defs' ->
+      app_ctx (Efun1_c defs c) (Efun defs' e) e1 ->
+      app_ctx (Efun1_c defs'' c) e e2 ->
+      hoist_rw e1 e2.
+
+(** reflexive transitive closure, parametrized by the 
+    number of steps for induction *)
+Inductive hoist_star_n : nat -> relation exp :=
+| hoistn_step :
+    forall e1 e2 e3 n, hoist_rw e1 e2 ->
+                  hoist_star_n n e2 e3 ->
+                  hoist_star_n (S n) e1 e3
+| hoistn_refl :
+    forall e, hoist_star_n 0 e e.
+
+Definition hoist_star (e1 e2: exp) : Prop :=
+  exists n, hoist_star_n n e1 e2.
+
+(** Hoisting normal form *)
+Definition hoist_nf (e : exp) :=
+  ~ exists e', hoist_rw e e'.
+
+(** easy lemmas about split_fds. 
+    TODO move split_fds in common file along with lemmas *)
+Lemma split_fds_nil_l fdefs : split_fds fdefs Fnil fdefs.
+  induction fdefs; constructor; eauto.
+Qed.
+
+Lemma split_fds_nil_r fdefs : split_fds Fnil fdefs fdefs.
+  induction fdefs; constructor; eauto.
+Qed.
+
+
+(* to do proofs simultaneously. TODO move to exp.v *)
+Lemma exp_def_mutual_ind :
+  forall (P : exp -> Prop) (P0 : fundefs -> Prop),
+    (forall (v : var) (t : type) (t0 : tag) (l : list var) (e : exp),
+       P e -> P (Econstr v t t0 l e)) ->
+    (forall (v : var) (l : list (tag * var)), P (Ecase v l)) ->
+    (forall (v : var) (t : type) (n : N) (v0 : var) (e : exp),
+       P e -> P (Eproj v t n v0 e)) ->
+    (forall f2 : fundefs, P0 f2 -> forall e : exp, P e -> P (Efun f2 e)) ->
+    (forall (v : var) (l : list var), P (Eapp v l)) ->
+    (forall (v : var) (t : type) (p : prim) (l : list var) (e : exp),
+       P e -> P (Eprim v t p l e)) ->
+    (forall (v : var) (t : type) (l : list var) (e : exp),
+       P e -> forall f5 : fundefs, P0 f5 -> P0 (Fcons v t l e f5)) ->
+    P0 Fnil -> (forall e : exp, P e) /\ (forall f : fundefs, P0 f).
+Proof.
+  intros. split.
+  apply (exp_mut P P0); assumption.
+  apply (fundefs_mut P P0); assumption.
+Qed.
+
+(** name the induction hypotheses only *)
+Ltac exp_defs_induction IH1 IH2 :=
+  apply exp_def_mutual_ind;
+  [ intros ? ? ? ? ? IH1 
+  | intros ? ?
+  | intros ? ? ? ? ? IH1
+  | intros ? IH2 ? IH1 
+  | intros ? ?
+  | intros ? ? ? ? ? IH1 
+  | intros ? ? ? ? IH1 ? IH2
+  | ].
+
+
+Definition injective {A B} (f : A -> B) :=
+  forall x y, f x = f y -> x = y.
+
+Lemma injective_comp {A B C} (f : A -> B) (g : B -> C) :
+  injective f -> injective g ->
+  injective (fun x => g (f x)).
+Proof.
+  unfold injective; eauto.
+Qed.
+
+Lemma exp_fundefs_hoist_no_fun:
+  (forall e,
+   exists g e',
+     (forall defs f,
+        exp_hoist e defs f = Efun (g defs) (f e')) /\
+     injective g /\
+     (forall defs, no_fun_defs defs -> no_fun_defs (g defs)) /\
+     no_fun e') /\
+  (forall defs,
+   exists g,
+     (forall hdefs f,
+        fundefs_hoist defs hdefs f = f (g hdefs)) /\
+     injective g /\
+     forall defs, no_fun_defs defs -> no_fun_defs (g defs)).
+Proof.
+  exp_defs_induction IHe IHf;
+  intros; try edestruct IHe as [g1 [? [H1 [H2 [H3 H4]]]]];
+  try edestruct IHf as [g2 [H5 [H6 H7]]];
+  try (now do 2 eexists; 
+       simpl; split; [ intros defs f; rewrite H1; eauto | split; eauto ]);
+  try (now exists id; repeat eexists; intros; unfold injective; eauto). 
+  simpl. exists (fun x => g1 (g2 x)); eexists.
+  split; intros. rewrite H1, H5; eauto.
+  split; eauto using injective_comp.
+  simpl. exists (fun d => Fcons v t l x (g2 (g1 d))). split.
+  intros; simpl. rewrite H1, H5; eauto. 
+  split; eauto using injective_comp. 
+  eapply injective_comp; eauto using injective_comp.
+  intros x1 x2 Heq; inv Heq; eauto.
+Qed.
+
+Corollary exp_hoist_head_no_fun e :
+  exists e' g,
+    (forall defs f, exp_hoist e defs f = Efun (g defs) (f e')) /\
+    no_fun e'.
+Proof.
+  destruct exp_fundefs_hoist_no_fun as [H1 _].
+  destruct (H1 e) as [? [? H2]]. do 2 eexists.
+  split; eapply H2; eauto.
+Qed.
+
+Corollary exp_hoist_head e :
+  exists e' g,
+    forall defs f, exp_hoist e defs f = Efun (g defs) (f e').
+Proof.
+  destruct exp_fundefs_hoist_no_fun as [H1 _].
+  destruct (H1 e) as [? [? H2]]. do 2 eexists. 
+  intros; eapply H2; eauto.
+Qed.
+
+Lemma exp_hoist_f_comp :
+  forall e e' defs hdefs f1 f2,
+    exp_hoist e defs f1 = Efun hdefs (f1 e') ->
+    exp_hoist e defs (fun x => f2 (f1 x)) = Efun hdefs (f2 (f1 e')).
+Proof.
+  intros e e' defs defs' g g' H.
+  destruct (exp_hoist_head e) as [e'' [g'' H']].
+  rewrite H' in H. inv H.
+  rewrite H'. eauto.
+Qed.
+
+
+Lemma app_ctx_fuse:
+  forall (c c' : exp_ctx) (e1 e2 e3 : exp),
+    app_ctx c e1 e2 ->
+    app_ctx c' e2 e3 ->
+    app_ctx (comp_ctx_f c' c) e1 e3.
+Proof.
+  intros c c' e1 e2 e3 H1 H2. rewrite <- app_ctx_f_correct.
+  rewrite <- app_ctx_f_fuse.
+  rewrite <- app_ctx_f_correct in H1, H2. rewrite H1. eauto.
+Qed.
+
+Lemma hoist_star_0 :
+  forall e e', hoist_star_n 0 e e' -> e = e'.
+Proof.
+  assert (H : 0%nat = 0%nat) by reflexivity.
+  revert H. generalize 0%nat at 1 3.
+  intros n  Heq e e' H. induction H; eauto; subst. congruence.
+Qed.
+
+Lemma hoist_star_n_trans n m e1 e2 e3:
+  hoist_star_n n e1 e2 ->
+  hoist_star_n m e2 e3 ->
+  hoist_star_n (n+m) e1 e3.
+Proof.
+  intros H1 H2. induction H1; eauto.
+  econstructor 1; eauto.
+Qed.
+
+Lemma hoist_star_trans e1 e2 e3:
+  hoist_star e1 e2 ->
+  hoist_star e2 e3 ->
+  hoist_star e1 e3.
+Proof.
+  intros [n H1] [m H2].
+  assert (H := hoist_star_n_trans n m e1 e2 e3 H1 H2).
+  eexists; eauto.
+Qed.
+
+Definition is_exp_ctx_f (f : exp -> exp) :=
+  exists c, forall e, app_ctx_f c e = f e.
+
+Definition is_def_ctx_f (h : exp -> fundefs) :=
+  exists c, forall e, app_f_ctx_f c e = h e.
+
+Definition is_def_ctx_defs (f : fundefs -> fundefs) := 
+  forall h, is_def_ctx_f h -> is_def_ctx_f (fun e => f (h e)).
+
+Lemma is_exp_ctx_f_comp (f1 f2 : exp -> exp) :
+  is_exp_ctx_f f1 -> is_exp_ctx_f f2 ->
+  is_exp_ctx_f (fun x => f1 (f2 x)).
+Proof.
+  intros [c1 H1] [c2 H2].
+  eexists (comp_ctx_f c1 c2). intros e.
+  rewrite <- app_ctx_f_fuse. rewrite H1. f_equal; eauto.
+Qed.
+
+Lemma is_def_ctx_f_comp f1 f2 :
+  is_def_ctx_defs f1 -> is_def_ctx_f f2 ->
+  is_def_ctx_f (fun x => f1 (f2 x)).
+Proof.
+  eauto.
+Qed.
+
+Lemma is_exp_ctx_f_defs f e :
+  is_def_ctx_f f -> 
+  is_exp_ctx_f (fun x : exp => Efun (f x) e).
+Proof.
+  intros [c1 H1].
+  eexists (Efun2_c c1 e). intros e1. simpl.
+  f_equal; eauto.
+Qed.
+
+(** hoisting is in the reflexive transitive closure of the rewrite relation *)
+Lemma exp_fundefs_hoist_in_hoist_star :
+  (forall e defs f,
+     is_exp_ctx_f f -> 
+     hoist_star (Efun defs (f e)) (exp_hoist e defs f)) /\
+  (forall defs e hdefs f g,
+     (forall d, no_fun_defs d -> no_fun_defs (f d)) ->
+     is_exp_ctx_f g ->
+     is_def_ctx_defs f ->
+     (forall d1 d2 d,
+        split_fds d1 d2 d ->
+        split_fds d1 (f d2) (f d)) ->
+     hoist_star (Efun hdefs (g (Efun (f defs) e)))
+                (Efun (fundefs_hoist defs hdefs f) (g e))).
+Proof.
+  apply exp_def_mutual_ind;
+  [intros x typ tag ys e IHe  fdefs f Hctx | intros x t_ys  fdefs f Hctx
+   | intros x typ n y e IHe fdefs f Hctx | intros defs IHdefs e IHe fdefs f Hctx
+   | intros g xs fdefs f Hctx
+   | intros x  typ pr ys e IHe fdefs f Hctx
+   | intros g typ xs e IHe defs IHdefs e' hdefs f h Hnf Hctx Hctx' Hsp
+   | intros e' hdefs f h Hnf Hctx Hctx' Hsp].
+  - simpl.
+    specialize (IHe fdefs (fun e => f (Econstr x typ tag ys e))).
+    apply IHe.
+    destruct Hctx as [c Hctx].
+    eexists (comp_ctx_f c (Econstr_c x typ tag ys Hole_c)).
+    intros e'. rewrite <- Hctx. now rewrite <- app_ctx_f_fuse. 
+  - eexists. apply hoistn_refl.
+  - simpl. specialize (IHe fdefs (fun e => f (Eproj x typ n y e))).
+    apply IHe.
+    destruct Hctx as [c Hctx].
+    eexists (comp_ctx_f c (Eproj_c x typ n y Hole_c)).
+    intros e'. rewrite <- Hctx. now rewrite <- app_ctx_f_fuse.
+  - simpl. specialize (IHe (fundefs_hoist defs fdefs id) f).
+    eapply hoist_star_trans; eauto. 
+    specialize (IHdefs e fdefs id f). eapply IHdefs; eauto.
+    unfold is_def_ctx_defs; eauto.
+  - eexists. apply hoistn_refl.
+  - simpl. specialize (IHe fdefs (fun e => f (Eprim x typ pr ys e))).
+    apply IHe.
+    destruct Hctx as [c Hctx].
+    eexists (comp_ctx_f c (Eprim_c x typ pr ys Hole_c)).
+    intros e'. rewrite <- Hctx. now rewrite <- app_ctx_f_fuse.
+  - simpl. destruct (exp_hoist_head_no_fun e) as [e1 [g' [H1 H2]]]. rewrite H1.
+    specialize (IHe hdefs (fun e => h (Efun (f (Fcons g typ xs e defs)) e'))).
+    rewrite H1 in IHe; simpl in *.     
+    specialize
+      (IHdefs e' (g' hdefs) (fun defs => f (Fcons g typ xs e1 defs)) h).
+    simpl in *.
+    eapply hoist_star_trans; [ eapply IHe | eapply IHdefs ]; eauto.
+    apply is_exp_ctx_f_comp; eauto.
+    eapply is_exp_ctx_f_defs with (f := fun x => f (Fcons g typ xs x defs)).
+    eapply Hctx'. exists (Fcons1_c g typ xs Hole_c defs).
+    intros; eauto. intros. 
+    intros g1 [c Hg1]. eapply is_def_ctx_f_comp; eauto.
+    exists (Fcons2_c g typ xs e1 c). intros; simpl; f_equal; eauto.
+    intros d1 d2 d Hds. eapply Hsp. constructor; eauto.
+  - simpl. eexists. econstructor 1; [| econstructor 2].
+    destruct Hctx as [c Hctx].
+    eapply hoist1 with (defs := hdefs) (defs' := f Fnil); eauto.
+    eapply Hsp. apply split_fds_nil_l.
+    apply app_ctx_f_correct. simpl. f_equal; eauto.
+    apply app_ctx_f_correct. simpl. f_equal; eauto.
+Qed.
